Add lifting implementation and well-typedness theorem.
Reveal semantics and correctness of lifting are not included yet.

theories/base.v
@@ -22,6 +22,20 @@ Section trans_ext.
 
 End trans_ext.
 
+(** * Classes *)
+Class FinMapPack K M := {
+  pack_finmap_decision :> EqDecision K | 0;
+  pack_finmap_fmap :> FMap M | 0;
+  pack_finmap_lookup :> ∀ A, Lookup K A (M A) | 0;
+  pack_finmap_empty :> ∀ A, Empty (M A) | 0;
+  pack_finmap_partial_alter :> ∀ A, PartialAlter K A (M A) | 0;
+  pack_finmap_omap :> OMap M | 0;
+  pack_finmap_merge :> Merge M | 0;
+  pack_finmap_to_list :> ∀ A, FinMapToList K A (M A) | 0;
+
+  pack_finmap :> FinMap K M | 0;
+}.
+
 (** * Lemmas *)
 
 Lemma insert_fresh_subseteq `{FinMapDom K M D} {A} k (m : M A) v :
