theories/lang_oadt/base.v
@@ -1,4 +1,5 @@
 From oadt Require Export prelude.
+From stdpp Require Import gmap.
 
 Export atom_instance.
 
@@ -13,6 +14,19 @@ Opaque aset.
 
 #[global]
 Opaque is_atom.
+
+Definition aamap := gmap (atom * atom).
+Instance aamap_is_finmap : FinMapPack (atom * atom) aamap.
+Proof.
+  esplit.
+  typeclasses eauto.
+Defined.
+
+#[global]
+Opaque aamap.
+
+#[global]
+Opaque aamap_is_finmap.
 
 Declare Custom Entry oadt.
 Declare Custom Entry oadt_def.
