theories/lang_oadt/lifting.v
@@ -1,0 +1,557 @@
+From oadt Require Import lang_oadt.base.
+From oadt Require Import lang_oadt.syntax.
+From oadt Require Import lang_oadt.semantics.
+From oadt Require Import lang_oadt.typing.
+From oadt Require Import lang_oadt.infrastructure.
+From oadt Require Import lang_oadt.admissible.
+From oadt Require Import lang_oadt.inversion.
+From oadt Require Import lang_oadt.preservation.
+
+Import syntax.notations.
+Import semantics.notations.
+Import typing.notations.
+
+Implicit Types (b : bool) (x X y Y : atom) (L : aset).
+
+#[local]
+Coercion EFVar : atom >-> expr.
+
+(** * Definitions *)
+
+(** ** Section and retraction context (Δ) *)
+(** Map ADT and OADT pair to section and retraction functions. *)
+Notation srctx := (aamap (atom * atom)).
+
+Definition srctx_wf (Σ : gctx) : srctx -> Prop :=
+  map_Forall (fun '(X, X') '(s, r) =>
+                exists τ τk e se re,
+                  Σ !! X = Some (DADT τ) /\
+                  Σ !! X' = Some (DOADT τk e) /\
+                  Σ !! s = Some (DFun (⊥, <{ Π:τk, Π~:(gvar X), (gvar X') (bvar 1) }>)
+                                 se) /\
+                  Σ !! r = Some (DFun (⊤, <{ Π:τk, Π~:((gvar X') (bvar 0)), gvar X }>)
+                                 re)).
+
+(* Destructive *)
+Ltac apply_srctx_wf :=
+  match goal with
+  | Hwf : srctx_wf _ ?Δ, H : ?Δ !! _ = Some _ |- _ =>
+    apply Hwf in H; try simp_hyp H
+  end.
+
+Section lifting.
+
+Context (Σ : gctx).
+Context (Hwf : gctx_wf Σ).
+Context (Δ : srctx).
+Context (Hsrwf : srctx_wf Σ Δ).
+
+Notation "e '-->!' e'" := (step Σ e e') (at level 40,
+                                         e' custom oadt at level 0).
+
+Notation "e '-->*' e'" := (clos_refl_trans_1n _ (step Σ) e e')
+                            (at level 40,
+                             e' custom oadt at level 0).
+
+Notation "Γ '⊢' e ':{' l '}' τ" := (typing Σ Γ e l τ)
+                                     (at level 40,
+                                      e custom oadt at level 99,
+                                      l constr at level 99,
+                                      τ custom oadt at level 99,
+                                      format "Γ  '⊢'  e  ':{' l '}'  τ").
+
+Notation "Γ '⊢' τ '::' κ" := (kinding Σ Γ τ κ)
+                               (at level 40,
+                                τ custom oadt at level 99,
+                                κ custom oadt at level 99).
+
+(** ** Generalized section *)
+(** Compute the section of [e] from public type [τ] to oblivious type [τ']. [e]
+is assumed a [body]. Alternatively, we may assume [e] is locally closed, and
+open/close the expressions accordingly. That way we also need to record the used
+atoms in an extra arguments, similar to the lifting functions below. *)
+Fixpoint gsec (τ τ' : expr) (e : expr) : option expr :=
+  match τ, τ' with
+  | <{ 𝟙 }>, <{ 𝟙 }> => Some <{ tape e }>
+  | <{ 𝔹 }>, <{ ~𝔹 }> => Some <{ tape (s𝔹 e) }>
+  | <{ τ1 * τ2 }>, <{ τ1' * τ2' }> =>
+    e1 <- gsec τ1 τ1' <{ π1 e }>;
+    e2 <- gsec τ2 τ2' <{ π2 e }>;
+    Some <{ (e1, e2) }>
+  | <{ τ1 + τ2 }>, <{ τ1' ~+ τ2' }> =>
+    e1 <- gsec τ1 τ1' <{ bvar 0 }>;
+    e2 <- gsec τ2 τ2' <{ bvar 0 }>;
+    Some <{ tape (case e of ~inl<τ1' ~+ τ2'> e1 | ~inr<τ1' ~+ τ2'> e2) }>
+  (* Outsource to predefined context *)
+  | <{ gvar X }>, <{ (gvar X') k }> =>
+    '(s, _) <- Δ !! (X, X');
+    Some <{ (gvar s) k e }>
+  | _, _ => None
+  end.
+
+(** ** Generalized retraction *)
+(** Compute the retraction of [e] from oblivious type [τ'] to public type [τ]. *)
+Fixpoint gret (τ τ' : expr) (e : expr) : option expr :=
+  match τ, τ' with
+  (* Unlike section, retraction also allows the oblivious type [τ'] to contain
+  non-oblivious components, as long as they match the corresponding components
+  in [τ]. *)
+  | <{ 𝟙 }>, <{ 𝟙 }> | <{ 𝔹 }>, <{ 𝔹 }> => Some e
+  | <{ gvar X }>, <{ gvar Y }> =>
+    if decide (X = Y) then Some e else None
+  | <{ Π:{_}_, _ }>, <{ Π:{_}_, _ }> =>
+    if decide (τ = τ') then Some e else None
+  | <{ 𝔹 }>, <{ ~𝔹 }> => Some <{ ~if tape e then true else false }>
+  | <{ τ1 * τ2 }>, <{ τ1' * τ2' }> =>
+    e1 <- gret τ1 τ1' <{ π1 e }>;
+    e2 <- gret τ2 τ2' <{ π2 e }>;
+    Some <{ (e1, e2) }>
+  | <{ τ1 + τ2 }>, <{ τ1' + τ2' }> =>
+    e1 <- gret τ1 τ1' <{ bvar 0 }>;
+    e2 <- gret τ2 τ2' <{ bvar 0 }>;
+    Some <{ case e of inl<τ1 + τ2> e1 | inr<τ1 + τ2> e2 }>
+  | <{ τ1 + τ2 }>, <{ τ1' ~+ τ2' }> =>
+    e1 <- gret τ1 τ1' <{ bvar 0 }>;
+    e2 <- gret τ2 τ2' <{ bvar 0 }>;
+    Some <{ ~case tape e of inl<τ1 + τ2> e1 | inr<τ1 + τ2> e2 }>
+  (* Outsource to predefined context *)
+  | <{ gvar X }>, <{ (gvar X') k }> =>
+    '(_, r) <- Δ !! (X, X');
+    Some <{ (gvar r) k e }>
+  | _, _ => None
+  end.
+
+(** ** Lifting *)
+
+(** The core lifting function. All arguments are supposed to be locally closed,
+and the indices in [τ'] have been instantiated with free variables in [xs]. [e]
+of type [τ] is lifted to the oblivious counterpart of type [τ']. [xs] keeps
+track of used free variables. *)
+Fixpoint lift_core (τ τ' : expr) (xs : aset) (e : expr) : option expr :=
+  match τ, τ' with
+  | <{ Π:{l}τ1, τ2 }>, <{ Π:{l'}τ1', τ2' }> =>
+    (* The function argument of [e] should accept retraction. *)
+    if decide (l = ⊤)
+    then let x := fresh xs in
+         r <- gret τ1 τ1' <{ fvar x }>;
+         (* [τ] and [τ'] are assumed non-dependent types, so [τ2] and [τ2']
+         are locally closed. *)
+         e' <- lift_core τ2 τ2' ({[x]} ∪ xs) <{ e r }>;
+         Some <{ \:{l'}τ1' => ,(close x e') }>
+    else None
+  | _, _ => gsec τ τ' e
+  end.
+
+(** This function handles type index arguments and calls [lift_core] to do the
+heavy lifting (pun intended). All arguments are locally closed. It lifts [e] of
+type [τ] to the oblivious counterpart of type [τ']. Unlike [lift_core], [τ']
+contains all the type index arguments from [τs]. *)
+Fixpoint lift_ (τ τ' : expr) (τs : list expr) (xs : aset) (e : expr) : option expr :=
+  match τs with
+  | _::τs =>
+    match τ' with
+    | <{ Π:{_}τ1, τ2' }> =>
+      let x := fresh xs in
+      e' <- lift_ τ <{ τ2'^x }> τs ({[x]} ∪ xs) e;
+      Some <{ \:τ1 => ,(close x e') }>
+    | _ => None
+    end
+  | [] => lift_core τ τ' xs e
+  end.
+
+(** The top level lifting function. It lifts [e] of type [τ] to the oblivious
+counterpart of type [τ'], whose public indices are [τs]. *)
+Definition lift (τ τ' : expr) (τs : list expr) (e : expr) : option expr :=
+  lift_ τ τ' τs ∅ e.
+
+(** Well-formedness of lifting input *)
+
+(** [τ] is not a dependent type (at top level). It may still take a higher-order
+function that is dependent type. *)
+Fixpoint nodep (τ : expr) : Prop :=
+  match τ with
+  | <{ Π:{_}_, τ2 }> =>
+    lc τ2 /\ nodep τ2
+  | _ => True
+  end.
+
+(** [lift_type_wf τs τ'] means [τ'] is a valid lifted oblivious type with
+indices [τs]. First, [τs] should be the "prefix" of [τ'], i.e. [τ'] is of the
+form [Π:τ1, Π:τ2, ..., τ] where [τs] is [τ1, τ2, ...]. Second, index types in
+[τs] are locally closed, i.e. there is no dependent type in indices. Third, the
+type with indices instantiated is non-dependent, i.e. [τ] should have the form
+[τ1 -> τ2 -> ...]. They can of course depend on the indices though. *)
+Inductive lift_type_wf : list expr -> expr -> Prop :=
+| LTVNil τ' : nodep τ' -> lift_type_wf [] τ'
+| LTVCons τk τs τ' L :
+    lc τk ->
+    (forall x, x ∉ L -> lift_type_wf τs <{ τ'^x }>) ->
+    lift_type_wf (τk::τs) <{ Π:τk, τ' }>
+.
+
+Instance list_expr_stale : Stale (list expr) := foldr (fun e S => fv e ∪ S) ∅.
+Arguments list_expr_stale /.
+
+(** * Theorems *)
+
+(** ** Well-typedness of section and retraction *)
+
+#[local]
+Set Default Proof Using "Type".
+
+Arguments open /.
+
+Ltac simpl_sr :=
+  intros; simpl in *; simplify_eq;
+  repeat (case_split; simpl in *; simplify_eq);
+  simplify_option_eq;
+  simp_hyps; intros; subst; simpl in *.
+
+Lemma gsec_body τ : forall τ' e e',
+  gsec τ τ' e = Some e' ->
+  lc τ' ->
+  body e ->
+  body e'.
+Proof.
+  unfold body, open.
+  induction τ; simpl_sr;
+      try solve [ eexists; simpl_cofin; eauto with lc ];
+      repeat apply_lc_inv;
+      (* Apply induction hypotheses. *)
+      repeat match goal with
+             | IH : context [gsec ?τ _ _ = _ -> _], H : gsec ?τ _ _ = _ |- _ =>
+               apply IH in H; clear IH
+             end;
+      simpl;
+      eauto using lc;
+      simp_hyps;
+      eexists; simpl_cofin;
+        try solve [ repeat econstructor; eauto; by rewrite open_lc ].
+
+  econstructor.
+  econstructor; eauto;
+    simpl_cofin; simpl;
+      repeat econstructor;
+      try solve [ repeat (rewrite open_lc; eauto) ];
+      rewrite open_comm by eauto using lc;
+      rewrite open_lc; eauto with lc.
+
+  Unshelve.
+  all: exact ∅.
+Qed.
+
+Lemma gsec_open τ s : forall τ' e e',
+  gsec τ τ' e = Some e' ->
+  lc τ' ->
+  gsec τ τ' <{ e^s }> = Some <{ e'^s }>.
+Proof.
+  unfold open.
+  induction τ; simpl_sr; eauto;
+    repeat apply_lc_inv;
+    repeat f_equal; try solve [ by rewrite !open_lc by eauto ].
+
+  repeat match goal with
+         | IH : context [gsec ?τ _ _ = _ -> _], H : gsec ?τ _ _ = _ |- _ =>
+           apply IH in H; clear IH; [ simpl in H; rewrite H | .. ]
+         end;
+    eauto.
+
+  all: rewrite open_body; eauto using gsec_body, body_bvar.
+Qed.
+
+Lemma gsec_type_correct τ : forall τ' e e' Γ κ κ',
+  gsec τ τ' e = Some e' ->
+  Γ ⊢ τ :: κ ->
+  Γ ⊢ τ' :: κ' ->
+  Γ ⊢ e :{⊤} τ ->
+  Γ ⊢ e' :{⊥} τ'.
+Proof using Hsrwf.
+  induction τ; simpl_sr;
+    eauto using typing, kinding;
+    apply_kind_inv.
+  (* OADT application *)
+  - apply_srctx_wf. simplify_eq.
+    relax_typing_type.
+    econstructor; eauto.
+    relax_typing_type.
+    econstructor; eauto.
+    econstructor; eauto.
+    reflexivity.
+    simpl.
+    rewrite open_lc; eauto with lc.
+  (* Product *)
+  - econstructor;
+      try match goal with
+          | H : _ -> _ |- _ ⊢ _ :{_} _ =>
+            eapply H; eauto using kinding;
+              solve [ relax_typing_type; econstructor; eauto ]
+          end.
+    reflexivity.
+  (* Sum *)
+  - econstructor; eauto using kinding.
+    econstructor; eauto using kinding;
+        simpl; simpl_cofin;
+        match goal with
+        | |- context [<{ ?τ1 ~+ ?τ2 }>] =>
+          rewrite open_lc with (e := τ1) by eauto with lc;
+            rewrite open_lc with (e := τ2) by eauto with lc
+        end;
+        econstructor; eauto using kinding, kinding_weakening_insert;
+          match goal with
+          | IH : context [gsec ?τ _ _ = _ -> _],
+                 H : gsec ?τ ?τ' _ = _ |- _ ⊢ _:{_} ?τ' =>
+            eapply IH
+          end;
+          eauto using gsec_open, kinding_weakening_insert with lc;
+          simpl; econstructor; simplify_map_eq;
+            eauto using kinding_weakening_insert.
+Qed.
+
+Lemma gret_body τ : forall τ' e e',
+  gret τ τ' e' = Some e ->
+  lc τ ->
+  lc τ' ->
+  body e' ->
+  body e.
+Proof.
+  unfold body, open.
+  induction τ; simpl_sr;
+      try solve [ eexists; simpl_cofin; eauto with lc ];
+      repeat apply_lc_inv;
+      (* Apply induction hypotheses. *)
+      repeat match goal with
+             | IH : context [gret ?τ _ _ = _ -> _], H : gret ?τ _ _ = _ |- _ =>
+               apply IH in H; clear IH
+             end;
+      simpl;
+      eauto using lc;
+      simp_hyps;
+      eexists; simpl_cofin;
+        try solve [ repeat econstructor; eauto; by rewrite open_lc ].
+
+  all: econstructor; eauto using lc;
+    simpl_cofin; simpl;
+      repeat econstructor;
+      try solve [ repeat (rewrite open_lc; eauto) ];
+      rewrite open_comm by eauto using lc;
+      rewrite open_lc; eauto with lc.
+
+  Unshelve.
+  all: exact ∅.
+Qed.
+
+Lemma gret_open τ s : forall τ' e e',
+  gret τ τ' e' = Some e ->
+  lc τ ->
+  lc τ' ->
+  gret τ τ' <{ e'^s }> = Some <{ e^s }>.
+Proof.
+  unfold open.
+  induction τ; simpl_sr; eauto;
+    repeat apply_lc_inv;
+    repeat f_equal; try solve [ by rewrite !open_lc by eauto ].
+
+  repeat match goal with
+         | IH : context [gret ?τ _ _ = _ -> _], H : gret ?τ _ _ = _ |- _ =>
+           apply IH in H; clear IH; [ simpl in H; rewrite H | .. ]
+         end;
+    eauto.
+
+  all: repeat f_equal;
+    try solve [ by rewrite !open_lc by eauto ];
+    rewrite open_body; eauto using gret_body, body_bvar.
+Qed.
+
+Lemma gret_type_correct τ : forall τ' e e' Γ κ κ',
+  gret τ τ' e' = Some e ->
+  Γ ⊢ τ :: κ ->
+  Γ ⊢ τ' :: κ' ->
+  Γ ⊢ e' :{⊤} τ' ->
+  Γ ⊢ e :{⊤} τ.
+Proof using Hsrwf.
+  induction τ; simpl_sr;
+    eauto using typing, kinding;
+    apply_kind_inv.
+
+  (* OADT application *)
+  apply_srctx_wf. simplify_eq.
+  relax_typing_type.
+  econstructor; eauto.
+  relax_typing_type.
+  econstructor; eauto.
+  econstructor; eauto.
+  reflexivity.
+  reflexivity.
+
+  (* Product *)
+  econstructor;
+    try match goal with
+        | H : _ -> _ |- _ ⊢ _ :{_} _ =>
+          eapply H; eauto using kinding;
+            solve [ relax_typing_type; econstructor; eauto ]
+        end.
+  reflexivity.
+
+  (* Sum *)
+  all: econstructor; eauto using typing, kinding;
+    simpl; simpl_cofin;
+      match goal with
+      | |- context [<{ ?τ1 + ?τ2 }>] =>
+        rewrite open_lc with (e := τ1) by eauto with lc;
+          rewrite open_lc with (e := τ2) by eauto with lc
+      end;
+      econstructor; eauto using kinding, kinding_weakening_insert;
+        match goal with
+        | IH : context [gret ?τ _ _ = _ -> _] |- _ ⊢ _:{_} ?τ =>
+          eapply IH
+        end;
+        eauto using gret_open, kinding_weakening_insert with lc;
+        simpl; (eapply TConv; [ econstructor; simplify_map_eq | .. ];
+                eauto using kinding_weakening_insert; reflexivity).
+Qed.
+
+(** ** Properties of input well-formedness *)
+
+Lemma nodep_rename_ τ x y :
+  nodep <{ τ }> ->
+  nodep <{ {x↦y}τ }>.
+Proof.
+  induction τ; simpl; intros; eauto.
+  - case_decide; eauto.
+  - simp_hyps. eauto with lc.
+Qed.
+
+Lemma lift_type_wf_rename_ τs τ' x y :
+  x # τs ->
+  lift_type_wf τs τ' ->
+  lift_type_wf τs <{ {x↦y}τ' }>.
+Proof.
+  intros ?.
+  induction 1; intros; subst; simpl in *.
+  - econstructor. eauto using nodep_rename_.
+  - rewrite subst_fresh.
+    econstructor; eauto.
+    simpl_cofin.
+    rewrite <- subst_open_comm; eauto using lc.
+    auto_eapply.
+    all: fast_set_solver!!.
+Qed.
+
+Lemma lift_type_wf_rename τs τ' x y :
+  x # τs ->
+  x # τ' ->
+  lift_type_wf τs <{ τ'^x }> ->
+  lift_type_wf τs <{ τ'^y }>.
+Proof.
+  intros.
+  rewrite (subst_intro τ' y x) by auto.
+  eauto using lift_type_wf_rename_.
+Qed.
+
+
+(** Well-typedness of lifting *)
+
+#[local]
+Set Default Proof Using "All".
+
+Arguments gret : simpl never.
+Arguments gsec : simpl never.
+
+Lemma lift_core_type_correct τ : forall τ' xs e e' κ' Γ,
+  lift_core τ τ' xs e = Some e' ->
+  nodep τ ->
+  nodep τ' ->
+  dom aset Γ ∪ tctx_fv Γ ⊆ xs ->
+  Γ ⊢ τ' :: κ' ->
+  Γ ⊢ e :{⊤} τ ->
+  Γ ⊢ e' :{⊥} τ'.
+Proof.
+  induction τ; simpl; intros;
+    apply_regularity;
+    eauto using gsec_type_correct.
+
+  case_split; simplify_eq.
+  case_decide; simplify_eq.
+  simplify_option_eq.
+  simp_hyps.
+  apply_kind_inv*. subst.
+  pose proof (atom_is_fresh xs).
+
+  match goal with
+  | IH : context[ lift_core _ _ _ _ = _ -> _ ], H : lift_core _ _ _ _ = _ |- _ =>
+    eapply IH in H
+  end; eauto; try set_shelve.
+  - typing_intro; eauto; try set_shelve.
+    rewrite open_close by eauto with lc.
+    rewrite open_lc_intro by auto.
+    eauto.
+  - simpl_cofin.
+    eapply_eq kinding_rename; eauto; try set_shelve.
+    by rewrite open_lc_intro by auto.
+  - relax_typing_type.
+    econstructor.
+    + eapply weakening_insert; eauto; try set_shelve.
+    + eapply gret_type_correct;
+        try (goal_is (_ ⊢ _ :: _); eapply kinding_weakening_insert);
+        eauto; try set_shelve.
+      eapply TConv.
+      econstructor. by simplify_map_eq.
+      eapply kinding_weakening_insert; eauto; try set_shelve.
+      reflexivity.
+      eapply kinding_weakening_insert; eauto; try set_shelve.
+      apply top_ub.
+    + by rewrite open_lc_intro.
+
+  Unshelve.
+  all: try fast_set_solver!!;
+           simpl_fv; rewrite ?close_fv by eauto with lc; try fast_set_solver*!!.
+Qed.
+
+Lemma lift_type_correct_ τ τs : forall τ' xs e e' κ' Γ,
+  lift_ τ τ' τs xs e = Some e' ->
+  nodep τ ->
+  lift_type_wf τs τ' ->
+  dom aset Γ ∪ tctx_fv Γ ⊆ xs ->
+  Γ ⊢ τ' :: κ' ->
+  Γ ⊢ e :{⊤} τ ->
+  Γ ⊢ e' :{⊥} τ'.
+Proof.
+  induction τs; simpl; intros.
+  - qauto use: lift_core_type_correct inv: lift_type_wf.
+  - case_split; simplify_eq.
+    simplify_option_eq.
+    select (lift_type_wf _ _) (fun H => sinvert H).
+    apply_kind_inv*. subst.
+    pose proof (atom_is_fresh xs).
+    simpl_cofin.
+    match goal with
+    | IH : context [lift_ ?τ _ _ _ _ = _ -> _], H : lift_ _ _ _ _ _ = _ |- _ =>
+      eapply IH in H
+    end; try set_shelve.
+    + typing_intro; eauto; try set_shelve.
+      rewrite open_close; eauto with lc.
+    + eauto.
+    + eauto using lift_type_wf_rename.
+    + eapply kinding_rename; eauto; try set_shelve.
+    + eapply weakening_insert; eauto; try set_shelve.
+
+  Unshelve.
+  all: try fast_set_solver!!;
+           simpl_fv; rewrite ?close_fv by eauto with lc; try fast_set_solver*!!.
+Qed.
+
+Theorem lift_type_correct τ τs τ' e e' κ :
+  lift τ τ' τs e = Some e' ->
+  nodep τ ->
+  lift_type_wf τs τ' ->
+  ∅ ⊢ τ' :: κ ->
+  ∅ ⊢ e :{⊤} τ ->
+  ∅ ⊢ e' :{⊥} τ'.
+Proof.
+  unfold lift.
+  intros.
+  eapply lift_type_correct_; eauto.
+  fast_set_solver!!.
+Qed.
+
+End lifting.
